src/asn1/RIoT.X509.AliasKeyCRT.fst
@@ -17,15 +17,15 @@ open LowParse.Spec.Bytes
 #push-options "--query_stats --z3rlimit 32 --fuel 4 --ifuel 4"
 type aliasKeyCRT_t (tbs_len: asn1_int32) = {
   aliasKeyCRT_tbs: B32.lbytes32 tbs_len;
-  aliasKeyCRT_sig_alg: algorithmIdentifier_t_inbound ED25519;
-  aliasKeyCRT_sig: x509_signature_t_inbound ED25519
+  aliasKeyCRT_sig_alg: algorithmIdentifier_t_inbound AlgID_Ed25519;
+  aliasKeyCRT_sig: x509_signature_t_inbound AlgID_Ed25519
 }
 #pop-options
 
 let aliasKeyCRT_t' (tbs_len: asn1_int32) = (
   (B32.lbytes32 tbs_len `tuple2`
-   algorithmIdentifier_t_inbound ED25519) `tuple2`
-   x509_signature_t_inbound ED25519
+   algorithmIdentifier_t_inbound AlgID_Ed25519) `tuple2`
+   x509_signature_t_inbound AlgID_Ed25519
 )
 
 let synth_aliasKeyCRT_t
@@ -49,9 +49,9 @@ let parse_aliasKeyCRT
 : parser _ (aliasKeyCRT_t tbs_len)
 = parse_flbytes32 tbs_len
   `nondep_then`
-  parse_algorithmIdentifier_sequence_TLV ED25519
+  parse_algorithmIdentifier_sequence_TLV AlgID_Ed25519
   `nondep_then`
-  parse_x509_signature_sequence_TLV ED25519
+  parse_x509_signature_sequence_TLV AlgID_Ed25519
   `parse_synth`
   synth_aliasKeyCRT_t tbs_len
 
@@ -61,15 +61,15 @@ let serialize_aliasKeyCRT
 = serialize_synth
   (* p1 *) (parse_flbytes32 tbs_len
             `nondep_then`
-            parse_algorithmIdentifier_sequence_TLV ED25519
+            parse_algorithmIdentifier_sequence_TLV AlgID_Ed25519
             `nondep_then`
-            parse_x509_signature_sequence_TLV ED25519)
+            parse_x509_signature_sequence_TLV AlgID_Ed25519)
   (* f2 *) (synth_aliasKeyCRT_t tbs_len)
   (* s1 *) (serialize_flbytes32 tbs_len
             `serialize_nondep_then`
-            serialize_algorithmIdentifier_sequence_TLV ED25519
+            serialize_algorithmIdentifier_sequence_TLV AlgID_Ed25519
             `serialize_nondep_then`
-            serialize_x509_signature_sequence_TLV ED25519)
+            serialize_x509_signature_sequence_TLV AlgID_Ed25519)
   (* g1 *) (synth_aliasKeyCRT_t' tbs_len)
   (* prf*) ()
 
@@ -80,48 +80,54 @@ let lemma_serialize_aliasKeyCRT_unfold
   serialize_aliasKeyCRT tbs_len `serialize` x ==
  (serialize_flbytes32 tbs_len `serialize` x.aliasKeyCRT_tbs)
   `Seq.append`
- (serialize_algorithmIdentifier_sequence_TLV ED25519 `serialize` x.aliasKeyCRT_sig_alg)
+ (serialize_algorithmIdentifier_sequence_TLV AlgID_Ed25519 `serialize` x.aliasKeyCRT_sig_alg)
   `Seq.append`
- (serialize_x509_signature_sequence_TLV ED25519 `serialize` x.aliasKeyCRT_sig)
+ (serialize_x509_signature_sequence_TLV AlgID_Ed25519 `serialize` x.aliasKeyCRT_sig)
 )
 = serialize_nondep_then_eq
   (* s1 *) (serialize_flbytes32 tbs_len)
-  (* s2 *) (serialize_algorithmIdentifier_sequence_TLV ED25519)
+  (* s2 *) (serialize_algorithmIdentifier_sequence_TLV AlgID_Ed25519)
   (* in *) (fst (synth_aliasKeyCRT_t' tbs_len x));
   serialize_nondep_then_eq
   (* s1 *) (serialize_flbytes32 tbs_len
             `serialize_nondep_then`
-            serialize_algorithmIdentifier_sequence_TLV ED25519)
-  (* s2 *) (serialize_x509_signature_sequence_TLV ED25519)
+            serialize_algorithmIdentifier_sequence_TLV AlgID_Ed25519)
+  (* s2 *) (serialize_x509_signature_sequence_TLV AlgID_Ed25519)
   (* in *) (synth_aliasKeyCRT_t' tbs_len x);
   serialize_synth_eq
   (* p1 *) (parse_flbytes32 tbs_len
             `nondep_then`
-            parse_algorithmIdentifier_sequence_TLV ED25519
+            parse_algorithmIdentifier_sequence_TLV AlgID_Ed25519
             `nondep_then`
-            parse_x509_signature_sequence_TLV ED25519)
+            parse_x509_signature_sequence_TLV AlgID_Ed25519)
   (* f2 *) (synth_aliasKeyCRT_t tbs_len)
   (* s1 *) (serialize_flbytes32 tbs_len
             `serialize_nondep_then`
-            serialize_algorithmIdentifier_sequence_TLV ED25519
+            serialize_algorithmIdentifier_sequence_TLV AlgID_Ed25519
             `serialize_nondep_then`
-            serialize_x509_signature_sequence_TLV ED25519)
+            serialize_x509_signature_sequence_TLV AlgID_Ed25519)
   (* g1 *) (synth_aliasKeyCRT_t' tbs_len)
   (* prf*) ()
   (* in *) x
 
 #restart-solver
-#push-options "--query_stats --z3rlimit 32" //--fuel 8 --ifuel 4"
+#push-options "--query_stats --z3rlimit 64 --fuel 4 --ifuel 4"
 let lemma_serialize_aliasKeyCRT_size
   (tbs_len: asn1_int32)
   (x: aliasKeyCRT_t tbs_len)
 : Lemma (
+  (* unfold *)
   length_of_opaque_serialization (serialize_aliasKeyCRT tbs_len) x ==
   length_of_opaque_serialization (serialize_flbytes32 tbs_len) x.aliasKeyCRT_tbs +
-  length_of_opaque_serialization (serialize_algorithmIdentifier_sequence_TLV ED25519) x.aliasKeyCRT_sig_alg +
-  length_of_opaque_serialization (serialize_x509_signature_sequence_TLV ED25519) x.aliasKeyCRT_sig
+  length_of_opaque_serialization (serialize_algorithmIdentifier_sequence_TLV AlgID_Ed25519) x.aliasKeyCRT_sig_alg +
+  length_of_opaque_serialization (serialize_x509_signature_sequence_TLV AlgID_Ed25519) x.aliasKeyCRT_sig /\
+  (* exact size *)
+  length_of_opaque_serialization (serialize_aliasKeyCRT tbs_len) x ==
+  v tbs_len + 76 // 7 + 69
 )
-= lemma_serialize_aliasKeyCRT_unfold tbs_len x
+= lemma_serialize_aliasKeyCRT_unfold tbs_len x;
+  (**) lemma_serialize_algorithmIdentifier_sequence_TLV_size_exact alg_AliasKey x.aliasKeyCRT_sig_alg;
+  (**) lemma_serialize_x509_signature_sequence_TLV_size_exact       alg_AliasKey x.aliasKeyCRT_sig
 #pop-options
 
 let aliasKeyCRT_t_inbound
@@ -143,17 +149,36 @@ let serialize_aliasKeyCRT_sequence_TLV
     (serialize_asn1_sequence_TLV (serialize_aliasKeyCRT tbs_len))
     ()
 
-let serialize_aliasKeyCRT_sequence_TLV_unfold
+let lemma_serialize_aliasKeyCRT_sequence_TLV_unfold
   (tbs_len: asn1_int32)
   (x: aliasKeyCRT_t_inbound tbs_len)
-: Lemma ( prop_serialize_asn1_sequence_TLV_unfold (serialize_aliasKeyCRT tbs_len) x )
+: Lemma ( predicate_serialize_asn1_sequence_TLV_unfold (serialize_aliasKeyCRT tbs_len) x )
 = lemma_serialize_asn1_sequence_TLV_unfold (serialize_aliasKeyCRT tbs_len) x
 
-let serialize_aliasKeyCRT_sequence_TLV_size
+let lemma_serialize_aliasKeyCRT_sequence_TLV_size
   (tbs_len: asn1_int32)
   (x: aliasKeyCRT_t_inbound tbs_len)
-: Lemma ( prop_serialize_asn1_sequence_TLV_size (serialize_aliasKeyCRT tbs_len) x )
+: Lemma ( predicate_serialize_asn1_sequence_TLV_size (serialize_aliasKeyCRT tbs_len) x )
 = lemma_serialize_asn1_sequence_TLV_size (serialize_aliasKeyCRT tbs_len) x
+
+#push-options "--query_stats --z3rlimit 64 --fuel 8 --ifuel 4"
+let lemma_serialize_aliasKeyCRT_sequence_TLV_size_exact
+  (tbs_len: asn1_int32)
+  (x: aliasKeyCRT_t_inbound tbs_len)
+: Lemma (
+  (* prove valid length *)
+  length_of_opaque_serialization (serialize_aliasKeyCRT tbs_len) x == v tbs_len + 76 /\
+  (* exact size *)
+  length_of_opaque_serialization (serialize_aliasKeyCRT_sequence_TLV tbs_len) x ==
+  v tbs_len + 77 + (length_of_asn1_length (u (v tbs_len + 76))) /\
+  (* upper bound *)
+  length_of_opaque_serialization (serialize_aliasKeyCRT_sequence_TLV tbs_len) x
+  <= v tbs_len + 84
+)
+= lemma_serialize_aliasKeyCRT_sequence_TLV_size tbs_len x;
+  (**) lemma_serialize_aliasKeyCRT_size tbs_len x
+#pop-options
+
 
 (* low *)
 
@@ -163,9 +188,9 @@ let serialize32_aliasKeyCRT_backwards
 = serialize32_synth_backwards
   (* s1 *) (serialize32_flbytes32_backwards tbs_len
             `serialize32_nondep_then_backwards`
-            serialize32_algorithmIdentifier_sequence_TLV_backwards ED25519
+            serialize32_algorithmIdentifier_sequence_TLV_backwards AlgID_Ed25519
             `serialize32_nondep_then_backwards`
-            serialize32_x509_signature_sequence_TLV_backwards ED25519)
+            serialize32_x509_signature_sequence_TLV_backwards AlgID_Ed25519)
   (* f2 *) (synth_aliasKeyCRT_t  tbs_len)
   (* g1 *) (synth_aliasKeyCRT_t' tbs_len)
   (* g1'*) (synth_aliasKeyCRT_t' tbs_len)
@@ -180,3 +205,29 @@ let serialize32_aliasKeyCRT_sequence_TLV_backwards
        (serialize32_aliasKeyCRT_backwards tbs_len))
     ()
 
+#restart-solver
+#push-options "--query_stats --z3rlimit 32 --fuel 4 --ifuel 4"
+let x509_get_AliasKeyCRT
+  (tbs_len: asn1_int32
+            { v tbs_len + 76 <= asn1_value_length_max_of_type SEQUENCE })
+  (aliasKeyCRT_tbs: B32.lbytes32 tbs_len)
+  (signature32: x509_signature_raw_t alg_AliasKey) // B32.lbytes32 64ul
+: Tot (aliasKeyCRT_t_inbound tbs_len)
+=
+  let aliasKeyCRT_sig_alg = x509_get_algorithmIdentifier alg_AliasKey in
+  (* Prf *) lemma_serialize_algorithmIdentifier_sequence_TLV_size_exact alg_AliasKey aliasKeyCRT_sig_alg;
+
+  let aliasKeyCRT_sig = x509_get_signature alg_AliasKey signature32 in
+  (* Prf *) lemma_serialize_x509_signature_sequence_TLV_size_exact alg_AliasKey aliasKeyCRT_sig;
+
+  let aliasKeyCRT: aliasKeyCRT_t tbs_len = {
+    aliasKeyCRT_tbs     = aliasKeyCRT_tbs;
+    aliasKeyCRT_sig_alg = aliasKeyCRT_sig_alg;
+    aliasKeyCRT_sig     = aliasKeyCRT_sig
+  } in
+  (* Prf *) lemma_serialize_aliasKeyCRT_unfold tbs_len aliasKeyCRT;
+  (* Prf *) lemma_serialize_aliasKeyCRT_size   tbs_len aliasKeyCRT;
+  (* Prf *) (**) lemma_serialize_flbytes32_size tbs_len aliasKeyCRT.aliasKeyCRT_tbs;
+
+(* return *) aliasKeyCRT
+#pop-options
