src/asn1/RIoT.X509.fst
@@ -31,6 +31,8 @@ module IB = LowStar.ImmutableBuffer
 module HS  = FStar.HyperStack
 module HST = FStar.HyperStack.ST
 
+module Ed25519 = Hacl.Ed25519
+
 let bytes_pub  = Seq.seq pub_uint8
 let lbytes_pub = Seq.lseq pub_uint8
 let bytes_sec  = Seq.seq uint8
@@ -38,408 +40,241 @@ let lbytes_sec = Seq.lseq uint8
 
 #restart-solver
 #push-options "--query_stats --z3rlimit 64 --initial_fuel 2 --initial_ifuel 2"
-let x509_get_aliasKey_crt_tbs_spec
+let x509_get_aliasKeyTBS_spec
+  (header_len: asn1_int32)
+  (aliasKeyTBS_header: lbytes_pub (v header_len))
+  (version: datatype_of_asn1_type INTEGER
+            { v header_len + length_of_asn1_primitive_TLV version + 155
+             <= asn1_value_length_max_of_type SEQUENCE })
   (fwid: lbytes_sec 32)
-  (riot_ver: datatype_of_asn1_type INTEGER)
   (deviceID_pub: lbytes_pub 32)
   (aliasKey_pub: lbytes_pub 32)
-  (aliasKey_crt_len: size_t)
-  (aliasKey_crt_pos: size_t { 0 <= v aliasKey_crt_pos /\
-                              v aliasKey_crt_pos <= v aliasKey_crt_len })
-  (aliasKey_crt: lbytes_pub (v aliasKey_crt_len))
-: GTot (s: bytes_pub { Seq.length s == v aliasKey_crt_pos + length_of_asn1_primitive_TLV riot_ver + 155 /\
-                       Seq.length s <= v aliasKey_crt_pos + 161 })
+// : GTot (s: bytes_pub { v header_len + length_of_asn1_primitive_TLV version + 155 <= asn1_value_length_max_of_type SEQUENCE /\
+//                        Seq.length s == v header_len + length_of_asn1_primitive_TLV version + 156 +
+//                                        length_of_asn1_length (u (v header_len + length_of_asn1_primitive_TLV version + 155))/\
+//                        Seq.length s <= v header_len + 167 })
+: GTot (aliasKeyTBS_t_inbound header_len)
 =
-  (* RIoT Extension *)
+  let aliasKeyTBS_header32: B32.lbytes32 header_len = B32.hide aliasKeyTBS_header in
   (*   Wrap `bytes` to `B32.bytes` *)
   let deviceID_pub32: B32.lbytes32 32ul = B32.hide deviceID_pub in
   let fwid32        : B32.lbytes32 32ul = B32.hide (declassify_secret_bytes fwid) in
-  (*   Construct `riot_extension` to serialize *)
-  let riot_extension    = x509_get_riot_extension riot_ver fwid32 deviceID_pub32 in
-  (*   Get serialization of `riot_extension` *)
-  let riot_extension_sx = serialize_riot_extension_sequence_TLV `serialize` riot_extension in
-  (* Prf *) lemma_serialize_riot_extension_sequence_TLV_size_exact riot_extension;
-
-  (* AliasKey SubjectPublicKeyInfo *)
   (*   Wrap `bytes` to `B32.bytes` *)
   let aliasKey_pub32: B32.lbytes32 32ul = B32.hide aliasKey_pub in
-  let aliasKey_pub_info    = x509_get_subjectPublicKeyInfo alg_AliasKey aliasKey_pub32 in
-  let aliasKey_pub_info_sx = serialize_subjectPublicKeyInfo_sequence_TLV alg_AliasKey `serialize` aliasKey_pub_info in
-  (* Prf *) lemma_serialize_subjectPublicKeyInfo_sequence_TLV_size_exact alg_AliasKey aliasKey_pub_info;
 
   (* AliasKey Certificate TBS *)
-  let aliasKey_crt_tbs = Seq.slice aliasKey_crt 0 (v aliasKey_crt_pos)
-                         `Seq.append`
-                         aliasKey_pub_info_sx
-                         `Seq.append`
-                         riot_extension_sx in
+  let aliasKeyTBS: aliasKeyTBS_t_inbound header_len = x509_get_AliasKeyTBS
+                                                        header_len
+                                                        aliasKeyTBS_header32
+                                                        version
+                                                        fwid32
+                                                        deviceID_pub32
+                                                        aliasKey_pub32 in
+  (* Prf *) lemma_serialize_aliasKeyTBS_size header_len aliasKeyTBS;
+  (* Prf *) lemma_serialize_aliasKeyTBS_sequence_TLV_size_exact header_len aliasKeyTBS;
 
-(* return *) aliasKey_crt_tbs
+aliasKeyTBS
+// (* return *) serialize_aliasKeyTBS_sequence_TLV header_len `serialize` aliasKeyTBS
 #pop-options
-
 
 let valid_ed25519_sign_mag_length
   (l: nat)
 = 64 + l <= max_size_t
 
-#push-options "--query_stats --z3rlimit 64 --fuel 4 --ifuel 4"
+(* ZT: Maybe FIXME: The large rlimit is required by the `modifies` clause. *)
+#restart-solver
+#push-options "--query_stats --z3rlimit 384 --fuel 10 --ifuel 6"
 let x509_get_aliasKey_crt_tbs
   (fwid: B.lbuffer uint8 32)
-  (riot_ver: datatype_of_asn1_type INTEGER)
+  (riot_version: datatype_of_asn1_type INTEGER)
   (deviceID_pub: B.lbuffer pub_uint8 32)
   (aliasKey_pub: B.lbuffer pub_uint8 32)
-  (aliasKey_crt_len: size_t)
-  (aliasKey_crt_pos: size_t { 0 <= v aliasKey_crt_pos /\
-                              v aliasKey_crt_pos <= v aliasKey_crt_len })
-  (aliasKey_crt: B.lbuffer pub_uint8 (v aliasKey_crt_len))
+  (aliasKeyTBS_header_len: size_t)
+  (aliasKeyTBS_header: B.lbuffer pub_uint8 (v aliasKeyTBS_header_len))
+  (aliasKeyTBS_len: size_t)
+  (aliasKeyTBS_buf: B.lbuffer pub_uint8 (v aliasKeyTBS_len))
 : HST.Stack unit
   (requires fun h ->
     B.(all_live h [buf fwid;
                    buf deviceID_pub;
                    buf aliasKey_pub;
-                   buf aliasKey_crt]) /\
+                   buf aliasKeyTBS_header;
+                   buf aliasKeyTBS_buf]) /\
     B.(all_disjoint [loc_buffer fwid;
                      loc_buffer deviceID_pub;
                      loc_buffer aliasKey_pub;
-                     loc_buffer aliasKey_crt]) /\
-    (* pre *) 0 <= v aliasKey_crt_pos /\ v aliasKey_crt_pos <= v aliasKey_crt_len /\
-    (* pre: buffer has enough space *)
-   (let            aliasKey_crt_tbs = x509_get_aliasKey_crt_tbs_spec
-                                        (B.as_seq h fwid)
-                                        (riot_ver)
-                                        (B.as_seq h deviceID_pub)
-                                        (B.as_seq h aliasKey_pub)
-                                        (aliasKey_crt_len)
-                                        (aliasKey_crt_pos)
-                                        (B.as_seq h aliasKey_crt) in
-     (* pre *) Seq.length (aliasKey_crt_tbs) <= v aliasKey_crt_len)
+                     loc_buffer aliasKeyTBS_header;
+                     loc_buffer aliasKeyTBS_buf]) /\
+    (* Pre *) v aliasKeyTBS_header_len + length_of_asn1_primitive_TLV riot_version + 155
+              <= asn1_value_length_max_of_type SEQUENCE /\
+    (* Pre *) v aliasKeyTBS_len
+              == v aliasKeyTBS_header_len +
+                 length_of_asn1_primitive_TLV riot_version +
+                 156 +
+                 length_of_asn1_length (u (v aliasKeyTBS_header_len + length_of_asn1_primitive_TLV riot_version + 155))
    )
   (ensures fun h0 _ h1 ->
+    let aliasKeyTBS: aliasKeyTBS_t_inbound aliasKeyTBS_header_len = x509_get_aliasKeyTBS_spec
+                                                                      (aliasKeyTBS_header_len)
+                                                                      (B.as_seq h0 aliasKeyTBS_header)
+                                                                      (riot_version)
+                                                                      (B.as_seq h0 fwid)
+                                                                      (B.as_seq h0 deviceID_pub)
+                                                                      (B.as_seq h0 aliasKey_pub) in
+    (* Prf *) lemma_serialize_aliasKeyTBS_sequence_TLV_size_exact aliasKeyTBS_header_len aliasKeyTBS;
+    (* Post *) B.(modifies (loc_buffer aliasKeyTBS_buf) h0 h1) /\
+    (* Post *) B.as_seq h1 aliasKeyTBS_buf == serialize_aliasKeyTBS_sequence_TLV aliasKeyTBS_header_len `serialize` aliasKeyTBS
+  )
+= let h0 = HST.get () in
+  HST.push_frame ();
+
+  let aliasKeyTBS_header = B.sub aliasKeyTBS_header 0ul aliasKeyTBS_header_len in
+  let aliasKeyTBS_header32: B32.lbytes32 aliasKeyTBS_header_len = B32.of_buffer aliasKeyTBS_header_len aliasKeyTBS_header in
+
+  let fwid_pub      : B.lbuffer pub_uint8 32 = B.alloca 0x00uy 32ul in
+  declassify_secret_buffer 32ul fwid fwid_pub;
+  let fwid_pub32        : B32.lbytes32 32ul = B32.of_buffer 32ul fwid_pub in
+
+  let deviceID_pub32: B32.lbytes32 32ul = B32.of_buffer 32ul deviceID_pub in
+  let aliasKey_pub32: B32.lbytes32 32ul = B32.of_buffer 32ul aliasKey_pub in
+
+  let aliasKeyTBS: aliasKeyTBS_t_inbound aliasKeyTBS_header_len = x509_get_AliasKeyTBS
+                                                                    aliasKeyTBS_header_len
+                                                                    aliasKeyTBS_header32
+                                                                    riot_version
+                                                                    fwid_pub32
+                                                                    deviceID_pub32
+                                                                    aliasKey_pub32 in
+
+  (* Prf *) lemma_serialize_aliasKeyTBS_sequence_TLV_size_exact aliasKeyTBS_header_len aliasKeyTBS;
+
+  let offset = serialize32_aliasKeyTBS_sequence_TLV_backwards
+                 aliasKeyTBS_header_len
+                 aliasKeyTBS
+                 aliasKeyTBS_buf
+                 aliasKeyTBS_len in
+
+  HST.pop_frame ()
+#pop-options
+
+// #push-options "--z3rlimit 16 --fuel 2 --ifuel 2"
+// let x509_get_aliasKey_crt_tbs_sig_sx_spec
+//   (deviceID_priv: lbytes_sec 32)
+//   (aliasKey_crt_tbs: bytes_pub {64 + Seq.length aliasKey_crt_tbs <= max_size_t})
+// : GTot (lbytes_pub 69)
+// =
+//   let aliasKey_crt_tbs_sec = classify_public_bytes aliasKey_crt_tbs in
+//   let aliasKey_crt_tbs_sig = Spec.Ed25519.sign deviceID_priv aliasKey_crt_tbs_sec in
+//   let aliasKey_crt_tbs_sig32 = B32.hide (declassify_secret_bytes aliasKey_crt_tbs_sig) in
+//   let aliasKey_crt_tbs_sig_bs = x509_get_signature AlgID_Ed25519 aliasKey_crt_tbs_sig32 in
+//   let aliasKey_crt_tbs_sig_sx = serialize_x509_signature_sequence_TLV AlgID_Ed25519
+//                                 `serialize`
+//                                 aliasKey_crt_tbs_sig_bs in
+//   (* Prf *) lemma_serialize_x509_signature_sequence_TLV_size_exact AlgID_Ed25519 aliasKey_crt_tbs_sig_bs;
+
+// (* return *) aliasKey_crt_tbs_sig_sx
+// #pop-options
+
+let () = ()
+
+#restart-solver
+#push-options "--query_stats --z3rlimit 32 --fuel 4 --ifuel 4"
+let x509_get_aliasKeyCRT_spec
+  (deviceID_priv: lbytes_sec 32)
+  (aliasKeyTBS_len: size_t
+                    { 64 + v aliasKeyTBS_len <= max_size_t /\
+                      v aliasKeyTBS_len + 76 <= asn1_value_length_max_of_type SEQUENCE })
+  (aliasKeyTBS_seq: lbytes_pub (v aliasKeyTBS_len))
+: GTot (aliasKeyCRT_t_inbound aliasKeyTBS_len)
+=
+
+  let aliasKeyTBS_seq32  : B32.lbytes32 aliasKeyTBS_len = B32.hide aliasKeyTBS_seq in
+
+  let aliasKeyTBS_seq_sec: lbytes_sec (v aliasKeyTBS_len) = classify_public_bytes aliasKeyTBS_seq in
+  let aliasKeyTBS_sig_sec: lbytes_sec 64 = Spec.Ed25519.sign deviceID_priv aliasKeyTBS_seq_sec in
+  let aliasKeyTBS_sig    : lbytes_pub 64 = declassify_secret_bytes aliasKeyTBS_sig_sec in
+  let aliasKeyTBS_sig32  : x509_signature_raw_t alg_AliasKey = B32.hide aliasKeyTBS_sig in
+
+  let aliasKeyCRT: aliasKeyCRT_t_inbound aliasKeyTBS_len = x509_get_AliasKeyCRT
+                                                             aliasKeyTBS_len
+                                                             aliasKeyTBS_seq32
+                                                             aliasKeyTBS_sig32 in
+
+(* return *) aliasKeyCRT
+#pop-options
+
+#restart-solver
+#push-options "--query_stats --z3rlimit 384 --fuel 10 --ifuel 6"
+let sign_and_finalize_aliasKeyCRT
+  (deviceID_priv: B.lbuffer uint8 32)
+  (aliasKeyTBS_len: size_t)
+  (aliasKeyTBS_buf: B.lbuffer pub_uint8 (v aliasKeyTBS_len))
+  (aliasKeyCRT_len: size_t)
+  (aliasKeyCRT_buf: B.lbuffer pub_uint8 (v aliasKeyCRT_len))
+: HST.Stack unit
+  (requires fun h ->
+    B.(all_live h [buf deviceID_priv;
+                   buf aliasKeyTBS_buf;
+                   buf aliasKeyCRT_buf]) /\
+    B.(all_disjoint [loc_buffer deviceID_priv;
+                     loc_buffer aliasKeyTBS_buf;
+                     loc_buffer aliasKeyCRT_buf]) /\
+    (* For `B.alloca` *)
+    0 < v aliasKeyTBS_len /\
+    (* For `Ed25519.sign` *)
+    64 + v aliasKeyTBS_len <= max_size_t /\
+    (* For `x509_get_aliasKeyCRT` *)
+    v aliasKeyTBS_len + 76 <= asn1_value_length_max_of_type SEQUENCE /\
+    (* `aliasKeyCRT_buf` has exact space to write serialization *)
+    v aliasKeyCRT_len
+    == v aliasKeyTBS_len + 77 + (length_of_asn1_length (u (v aliasKeyTBS_len + 76)))
+   )
+  (ensures fun h0 _ h1 ->
+    let aliasKeyCRT: aliasKeyCRT_t_inbound aliasKeyTBS_len = x509_get_aliasKeyCRT_spec
+                                                                      (B.as_seq h0 deviceID_priv)
+                                                                      (aliasKeyTBS_len)
+                                                                      (B.as_seq h0 aliasKeyTBS_buf) in
+    (* Prf *) lemma_serialize_aliasKeyCRT_sequence_TLV_size_exact aliasKeyTBS_len aliasKeyCRT;
+    (* Post *) B.(modifies (loc_buffer aliasKeyCRT_buf) h0 h1) /\
+    (* Post *) B.as_seq h1 aliasKeyCRT_buf == serialize_aliasKeyCRT_sequence_TLV aliasKeyTBS_len `serialize` aliasKeyCRT /\
     True
   )
 =
   HST.push_frame ();
 
-  (* RIoT Extension *)
-  (*   Wrap `bytes` to `B32.bytes` *)
-  let deviceID_pub32: B32.lbytes32 32ul = B32.of_buffer 32ul deviceID_pub in
-  let fwid_pub      : B.lbuffer pub_uint8 32 = B.alloca 0x00uy 32ul in
-  declassify_secret_buffer 32ul fwid fwid_pub;
-  let fwid_pub32        : B32.lbytes32 32ul = B32.of_buffer 32ul fwid_pub in
-  (*   Construct `riot_extension` to serialize *)
-  let riot_extension    = x509_get_riot_extension riot_ver deviceID_pub32 fwid_pub32 in
+  let aliasKeyTBS_buf32: B32.lbytes32 aliasKeyTBS_len = B32.of_buffer aliasKeyTBS_len aliasKeyTBS_buf in
 
-  let offset = serialize32_riot_extension_sequence_TLV_backwards
-                 riot_extension
-                 aliasKey_crt
-                 aliasKey_crt_len in
+  let aliasKeyTBS_buf_sec: B.lbuffer uint8 (v aliasKeyTBS_len) = B.alloca (u8 0x00) aliasKeyTBS_len in
+  classify_public_buffer
+    (* len *) aliasKeyTBS_len
+    (* src *) aliasKeyTBS_buf
+    (* dst *) aliasKeyTBS_buf_sec;
 
-  let aliasKey_pub32: B32.lbytes32 32ul = B32.of_buffer 32ul aliasKey_pub in
-  let aliasKey_pub_info    = x509_get_subjectPublicKeyInfo alg_AliasKey aliasKey_pub32 in
+  let aliasKeyTBS_sig_sec: B.lbuffer uint8 64 = B.alloca (u8 0x00) 64ul in
+  Ed25519.sign
+    (* sig *) aliasKeyTBS_sig_sec
+    (* key *) deviceID_priv
+    (* len *) aliasKeyTBS_len
+    (* msg *) aliasKeyTBS_buf_sec;
 
-  let offset = serialize32_subjectPublicKeyInfo_sequence_TLV_backwards
+  let aliasKeyTBS_sig: B.lbuffer pub_uint8 64 = B.alloca 0x00uy 64ul in
+  declassify_secret_buffer
+    (* len *) 64ul
+    (* src *) aliasKeyTBS_sig_sec
+    (* dst *) aliasKeyTBS_sig;
+  let aliasKeyTBS_sig32: x509_signature_raw_t alg_AliasKey = B32.of_buffer 64ul aliasKeyTBS_sig in
 
-                 aliasKey_pub_info
-                 aliasKey_crt
-                 (aliasKey_crt_len - offset) in
+  let aliasKeyCRT: aliasKeyCRT_t_inbound aliasKeyTBS_len = x509_get_AliasKeyCRT
+                                                             aliasKeyTBS_len
+                                                             aliasKeyTBS_buf32
+                                                             aliasKeyTBS_sig32 in
+  (* Prf *) lemma_serialize_aliasKeyCRT_sequence_TLV_size_exact aliasKeyTBS_len aliasKeyCRT;
+
+  let offset = serialize32_aliasKeyCRT_sequence_TLV_backwards
+                 aliasKeyTBS_len
+                 aliasKeyCRT
+                 aliasKeyCRT_buf
+                 aliasKeyCRT_len in
 
   HST.pop_frame ()
 #pop-options
-
-
-#push-options "--z3rlimit 16 --fuel 2 --ifuel 2"
-let x509_get_aliasKey_crt_tbs_sig_sx_spec
-  (deviceID_priv: lbytes_sec 32)
-  (aliasKey_crt_tbs: bytes_pub {64 + Seq.length aliasKey_crt_tbs <= max_size_t})
-: GTot (lbytes_pub 69)
-=
-  let aliasKey_crt_tbs_sec = classify_public_bytes aliasKey_crt_tbs in
-  let aliasKey_crt_tbs_sig = Spec.Ed25519.sign deviceID_priv aliasKey_crt_tbs_sec in
-  let aliasKey_crt_tbs_sig32 = B32.hide (declassify_secret_bytes aliasKey_crt_tbs_sig) in
-  let aliasKey_crt_tbs_sig_bs = x509_get_signature ED25519 aliasKey_crt_tbs_sig32 in
-  let aliasKey_crt_tbs_sig_sx = serialize_x509_signature_sequence_TLV ED25519
-                                `serialize`
-                                aliasKey_crt_tbs_sig_bs in
-  (* Prf *) lemma_serialize_x509_signature_sequence_TLV_size_exact ED25519 aliasKey_crt_tbs_sig_bs;
-
-(* return *) aliasKey_crt_tbs_sig_sx
-#pop-options
-
-#push-options "--z3rlimit 32 --initial_fuel 2 --initial_ifuel 2"
-let x509_get_aliasKey_crt_spec
-  (deviceID_priv: lbytes_sec 32)
-  (aliasKey_crt_tbs: bytes_pub {64 + Seq.length aliasKey_crt_tbs <= max_size_t})
-: GTot (aliasKey_crt: bytes_pub { Seq.length aliasKey_crt == Seq.length aliasKey_crt_tbs + 76 })
-=
-  let aliasKey_crt_tbs_sig_sx = x509_get_aliasKey_crt_tbs_sig_sx_spec
-                                  deviceID_priv
-                                  aliasKey_crt_tbs in
-  let aliasKey_crt_tbs_sig_algId = x509_get_algorithmIdentifier ED25519 in
-  let aliasKey_crt_tbs_sig_algId_sx = serialize_algorithmIdentifier_sequence_TLV ED25519
-                                      `serialize`
-                                      aliasKey_crt_tbs_sig_algId in
-  (* Prf *) lemma_serialize_algorithmIdentifier_sequence_TLV_size_exact ED25519 aliasKey_crt_tbs_sig_algId;
-
-  let aliasKey_crt = aliasKey_crt_tbs
-                     `Seq.append`
-                     aliasKey_crt_tbs_sig_algId_sx
-                     `Seq.append`
-                     aliasKey_crt_tbs_sig_sx in
-
-  // assert ( Seq.length aliasKey_crt ==
-  //          Seq.length aliasKey_crt_tbs +
-  //          Seq.length aliasKey_crt_tbs_sig_algId_sx +
-  //          Seq.length aliasKey_crt_tbs_sig_sx );
-
-(* return *) aliasKey_crt
-#pop-options
-
-(*)
-#restart-solver
-#push-options "--query_stats --z3rlimit 128 --fuel 16 --ifuel 4"
-let x509_get_riot_extension
-  (version: datatype_of_asn1_type INTEGER)
-  (deviceKeyPub: B32.lbytes32 32ul)
-  (fwid: B32.lbytes32 32ul)
-: Tot (x509_extension_t_inbound serialize_compositeDeviceID_sequence_TLV)
-=
-  let compositeDeviceID: compositeDeviceID_t_inbound = x509_get_compositeDeviceID version deviceKeyPub fwid in
-  (* Prf *) lemma_serialize_compositeDeviceID_sequence_TLV_size_exact compositeDeviceID;
-
-  let riot_extension: x509_extension_t serialize_compositeDeviceID_sequence_TLV = {
-    x509_extID       = OID_RIOT;
-    x509_extCritical = false;
-    x509_extValue    = compositeDeviceID
-  } in
-  (* Prf *) lemma_serialize_x509_extension_unfold
-            (* s *) serialize_compositeDeviceID_sequence_TLV
-            (* x *) riot_extension;
-  (* Prf *) lemma_serialize_x509_extension_size
-            (* s *) serialize_compositeDeviceID_sequence_TLV
-            (* x *) riot_extension;
-  (* Prf *) (**) lemma_serialize_asn1_oid_TLV_size riot_extension.x509_extID;
-  (* Prf *) (**) lemma_serialize_asn1_boolean_TLV_size riot_extension.x509_extCritical;
-  // assume (length_of_asn1_primitive_TLV riot_extension.x509_extID == 11); ()
-  // assume (length_of_asn1_primitive_TLV riot_extension.x509_extCritical == 3);
-  // assert_norm (length_of_asn1_primitive_TLV riot_extension.x509_extValue.riot_version <= 6);
-  // assert_norm (length_of_opaque_serialization serialize_fwid_sequence_TLV riot_extension.x509_extValue.riot_fwid == 47);
-  // (* Prf *) lemma_serialize_x509_extension_sequence_TLV_size
-  //           (* s *) serialize_compositeDeviceID_sequence_TLV
-  //           (* x *) riot_extension;
-
-(*return*) riot_extension
-#pop-options
-
-
-#push-options "--query_stats --z3rlimit 32 --fuel 8 --ifuel 4"
-let lemma_serialize_riot_extension_oid
-  (x: x509_extension_t serialize_compositeDeviceID_sequence_TLV)
-: Lemma (
-  // length_of_asn1_primitive_TLV x.x509_extID == 11
-  x.x509_extID == OID_RIOT
-)
-= ()
-
-let lemma_serialize_riot_extension_size_exact
-  (x: x509_extension_t serialize_compositeDeviceID_sequence_TLV)
-: Lemma (
-  length_of_opaque_serialization (serialize_x509_extension serialize_compositeDeviceID_sequence_TLV) x ==
-  length_of_asn1_primitive_TLV x.x509_extValue.riot_version + 109 // (93 +1+1) + 11 + 3 +1+1
-)
-= //lemma_serialize_x509_extension_sequence_TLV_size serialize_compositeDeviceID_sequence_TLV x;
-  lemma_serialize_x509_extension_size              serialize_compositeDeviceID_sequence_TLV x;
-  assert (length_of_opaque_serialization (serialize_x509_extension serialize_compositeDeviceID_sequence_TLV) x ==
-          length_of_asn1_primitive_TLV x.x509_extID +
-          length_of_asn1_primitive_TLV x.x509_extCritical +
-          length_of_TLV OCTET_STRING (length_of_opaque_serialization serialize_compositeDeviceID_sequence_TLV x.x509_extValue));
-  (**) lemma_serialize_asn1_oid_TLV_size                         x.x509_extID;
-  // (**) lemma_serialize_asn1_boolean_TLV_size                     x.x509_extCritical;
-  // (**) lemma_serialize_compositeDeviceID_sequence_TLV_size_exact x.x509_extValue;
-  assert (length_of_asn1_primitive_TLV x.x509_extID == 11);
-  admit();
-()
-#pop-options
-
-open Lib.IntTypes
-open RIoT.Base
-open RIoT.Declassify
-open Spec.Hash.Definitions
-
-let bytes_pub  = Seq.seq pub_uint8
-let lbytes_pub = Seq.lseq pub_uint8
-let bytes_sec  = Seq.seq uint8
-let lbytes_sec = Seq.lseq uint8
-
-
-#restart-solver
-#push-options "--query_stats --z3rlimit 256 --initial_fuel 8 --initial_ifuel 3"
-let x509_get_aliasKey_crt_tbs_spec
-  (cdi: lbytes_sec 32)
-  (fwid: lbytes_sec 32)
-  (riot_ver: datatype_of_asn1_type INTEGER)
-  (riot_label_DeviceID_len: size_t { (* for Hacl.HKDF.expand_st *)
-                                     hash_length alg + v riot_label_DeviceID_len + 1 + block_length alg < pow2 32 /\
-                                     (* for Spec.Aigle.HKDF.expand *)
-                                     hash_length alg + v riot_label_DeviceID_len + 1 + block_length alg < max_input_length alg })
-  (riot_label_DeviceID: lbytes_sec (v riot_label_DeviceID_len))
-  (aliasKey_crt_len: size_t)
-  (aliasKey_crt_pos: size_t { 0 <= v aliasKey_crt_pos /\
-                              v aliasKey_crt_pos <= v aliasKey_crt_len })
-  (aliasKey_crt: lbytes_pub (v aliasKey_crt_len))
-// : GTot (l: nat & lbytes_pub l)
-= let cdigest = Spec.Agile.Hash.hash alg cdi in
-  let deviceID_pub, deviceID_priv = riot_derive_key_pair_spec
-                                    (* ikm *) 32ul cdigest
-                                    (* lbl *) riot_label_DeviceID_len riot_label_DeviceID in
-  let adigest = Spec.Agile.HMAC.hmac alg cdigest fwid in
-  let aliasKey_pub, aliasKey_priv = riot_derive_key_pair_spec
-                                    (* ikm *) 32ul adigest
-                                    (* lbl *) riot_label_DeviceID_len riot_label_DeviceID in
-  let deviceID_pub32: B32.lbytes32 32ul = B32.hide deviceID_pub in
-  let fwid32: B32.lbytes32 32ul = B32.hide (declassify_secret_bytes 32 fwid) in
-  let riot_extension = x509_get_riot_extension riot_ver deviceID_pub32 fwid32 in
-  let riot_extension_sx = serialize_x509_extension_sequence_TLV serialize_compositeDeviceID_sequence_TLV
-                          `serialize`
-                          riot_extension in
-  (* AliasKey Certificate TBS *)
-  let aliasKey_crt_tbs = Seq.slice aliasKey_crt 0 (v aliasKey_crt_pos)
-                         `Seq.append` (* FIXME: Here, we need to require that `tbs`'s length is acceptable by the signing func *)
-                         riot_extension_sx in
-  // let _ = lemma_serialize_x509_extension_size serialize_compositeDeviceID_sequence_TLV riot_extension;
-  //         (**) lemma_serialize_asn1_oid_TLV_size riot_extension.x509_extID;
-  //         (**) lemma_serialize_asn1_boolean_TLV_size riot_extension.x509_extCritical;
-  //         (**) lemma_serialize_compositeDeviceID_sequence_TLV_size_exact riot_extension.x509_extValue;
-  //         lemma_serialize_x509_extension_sequence_TLV_size serialize_compositeDeviceID_sequence_TLV riot_extension in
-  // let aliasKey_crt_tbs = classify_public_bytes (Seq.length aliasKey_crt_tbs) aliasKey_crt_tbs in
-
-(* return *) (|Seq.length aliasKey_crt_tbs, aliasKey_crt_tbs|)
-
-// let _ = assert (length_of_oid OID_EC_GRP_SECP256R1 == 6)
-// let _ = assert (length_of_asn1_primitive_TLV (Mkbit_string_t 33ul 0ul (magic())) == 35)
-
-(*
-#push-options "--query_stats --z3rlimit 96 --initial_fuel 16 --max_fuel 32 --initial_ifuel 2"
-let x509_get_riot_extension
-  (version: datatype_of_asn1_type INTEGER)
-  (deviceKeyPub: B32.lbytes32 32ul)
-  (fwid: B32.lbytes32 32ul)
-: Tot (x509_extension_t_inbound serialize_compositeDeviceID_sequence_TLV)
-=
-  // lemma_serialize_asn1_oid_TLV_size OID_RIOT;
-  // assert (length_of_opaque_serialization serialize_asn1_oid_TLV OID_RIOT == 11);
-  // (* Prf *) (**) lemma_serialize_asn1_boolean_TLV_size false;
-  // assert (length_of_opaque_serialization serialize_asn1_boolean_TLV false == 3);
-  let deviceIDPublicKeyInfo: subjectPublicKeyInfo_t alg_DeviceID = x509_get_public_key_info alg_DeviceID deviceKeyPub in
-  (* Prf *) lemma_serialize_subjectPublicKeyInfo_unfold alg_DeviceID deviceIDPublicKeyInfo;
-  (* Prf *) lemma_serialize_subjectPublicKeyInfo_size alg_DeviceID deviceIDPublicKeyInfo;
-  (* Prf *)      lemma_serialize_algorithmIdentifier_unfold alg_DeviceID deviceIDPublicKeyInfo.subjectPubKey_alg;
-  (* Prf *)      (**) lemma_serialize_asn1_oid_TLV_size deviceIDPublicKeyInfo.subjectPubKey_alg.alg_id_oid_ecdsa;
-  (* Prf *)      (**) lemma_serialize_asn1_oid_TLV_size deviceIDPublicKeyInfo.subjectPubKey_alg.alg_id_oid_p256;
-  (* Prf *)      lemma_serialize_algorithmIdentifier_sequence_TLV_size alg_DeviceID deviceIDPublicKeyInfo.subjectPubKey_alg;
-  (* Prf *) (**) lemma_serialize_asn1_bit_string_TLV_size deviceIDPublicKeyInfo.subjectPubKey;
-  (* Prf *) lemma_serialize_subjectPublicKeyInfo_sequence_TLV_size alg_DeviceID deviceIDPublicKeyInfo;
-
-  let fwid: fwid_t = {
-    fwid_hashAlg = OID_DIGEST_SHA256;
-    fwid_value   = (|32ul, fwid|)
-  } in
-  (* Prf *) lemma_serialize_fwid_size fwid;
-  (* Prf *) (**) lemma_serialize_asn1_oid_TLV_size fwid.fwid_hashAlg;
-  (* Prf *) (**) lemma_serialize_asn1_octet_string_TLV_size fwid.fwid_value;
-  (* Prf *) lemma_serialize_fwid_sequence_TLV_size fwid;
-
-  let compositeDeviceID: compositeDeviceID_t = {
-    riot_version  = version;
-    riot_deviceID = deviceIDPublicKeyInfo;
-    riot_fwid     = fwid
-  } in
-  (* Prf *) lemma_serialize_compositeDeviceID_size compositeDeviceID;
-  (* Prf *) (**) lemma_serialize_asn1_integer_TLV_size compositeDeviceID.riot_version;
-  (* Prf *) lemma_serialize_compositeDeviceID_sequence_TLV_size compositeDeviceID;
-
-  let riot_extension: x509_extension_t serialize_compositeDeviceID_sequence_TLV = {
-    x509_extID       = OID_RIOT;
-    x509_extCritical = false;
-    x509_extValue    = compositeDeviceID
-  } in
-  (* Prf *) lemma_serialize_x509_extension_unfold
-            (* s *) serialize_compositeDeviceID_sequence_TLV
-            (* x *) riot_extension;
-  (* Prf *) lemma_serialize_x509_extension_size
-            (* s *) serialize_compositeDeviceID_sequence_TLV
-            (* x *) riot_extension;
-  (* Prf *) (**) lemma_serialize_asn1_oid_TLV_size riot_extension.x509_extID;
-  (* Prf *) (**) lemma_serialize_asn1_boolean_TLV_size riot_extension.x509_extCritical;
-  (* FIXME: ZT: They are true, but Z3 has trouble to prove them in a not small query. *)
-  assume (length_of_opaque_serialization serialize_asn1_oid_TLV riot_extension.x509_extID == 11);
-  assume (length_of_opaque_serialization serialize_asn1_boolean_TLV riot_extension.x509_extCritical == 3);
-  assume (length_of_opaque_serialization (serialize_x509_extension serialize_compositeDeviceID_sequence_TLV) riot_extension
-          <= asn1_length_max - 6);
-  (* Prf *) lemma_serialize_x509_extension_sequence_TLV_size
-            (* s *) serialize_compositeDeviceID_sequence_TLV
-            (* x *) riot_extension;
-(*return*) riot_extension
-#pop-options
-
-let _ = assert (length_of_oid OID_EC_GRP_SECP256R1 == 6)
-let _ = assert (length_of_asn1_primitive_TLV (Mkbit_string_t 33ul 0ul (magic())) == 35)
-
-(*)
-#restart-solver
-#push-options "--query_stats --z3rlimit 96 --initial_fuel 8 --initial_ifuel 2"// --initial_fuel 8 --max_fuel 16 --initial_ifuel 2"// 96 --max_fuel 16 --max_ifuel 16"
-let x509_get_riot_extension
-  (version: datatype_of_asn1_type INTEGER)
-  (deviceKeyPub: B32.lbytes32 32ul)
-  (fwid: B32.lbytes32 32ul)
-// : Tot (x509_extension_t_inbound serialize_compositeDeviceID_sequence_TLV)
-=
-  let compositeDeviceID = x509_get_compositeDeviceID
-                            version
-                            deviceKeyPub
-                            fwid in
-  (* Prf *) lemma_serialize_compositeDeviceID_unfold compositeDeviceID;
-  (* Prf *) lemma_serialize_compositeDeviceID_size   compositeDeviceID;
-                 (* version *)
-  (* Prf *) (**) lemma_serialize_asn1_integer_TLV_size compositeDeviceID.riot_version;
-  (* Prf *)      lemma_serialize_subjectPublicKeyInfo_unfold alg_DeviceID compositeDeviceID.riot_deviceID;
-  (* Prf *)      lemma_serialize_subjectPublicKeyInfo_size   alg_DeviceID compositeDeviceID.riot_deviceID;
-  (* Prf *)           lemma_serialize_algorithmIdentifier_unfold alg_DeviceID compositeDeviceID.riot_deviceID.subjectPubKey_alg;
-  (* Prf *)           lemma_serialize_algorithmIdentifier_size   alg_DeviceID compositeDeviceID.riot_deviceID.subjectPubKey_alg;
-  (* Prf *)           (**) lemma_serialize_asn1_oid_TLV_size compositeDeviceID.riot_deviceID.subjectPubKey_alg.alg_id_oid_ecdsa;
-  (* Prf *)           (**) lemma_serialize_asn1_oid_TLV_size compositeDeviceID.riot_deviceID.subjectPubKey_alg.alg_id_oid_p256;
-  (* Prf *)           lemma_serialize_algorithmIdentifier_sequence_TLV_size alg_DeviceID compositeDeviceID.riot_deviceID.subjectPubKey_alg;
-  (* Prf *)      (**) lemma_serialize_asn1_bit_string_TLV_size compositeDeviceID.riot_deviceID.subjectPubKey;
-  (* Prf *)      lemma_serialize_subjectPublicKeyInfo_sequence_TLV_unfold alg_DeviceID compositeDeviceID.riot_deviceID;
-                 (* fwid *)
-  (* Prf *)      lemma_serialize_fwid_unfold compositeDeviceID.riot_fwid;
-  (* Prf *)      lemma_serialize_fwid_size   compositeDeviceID.riot_fwid;
-  (* Prf *)      (**) lemma_serialize_asn1_oid_TLV_size compositeDeviceID.riot_fwid.fwid_hashAlg;
-  (* Prf *)      (**) lemma_serialize_asn1_octet_string_TLV_size compositeDeviceID.riot_fwid.fwid_value;
-  (* Prf *)      lemma_serialize_fwid_sequence_TLV_size compositeDeviceID.riot_fwid;
-  (* Prf *) lemma_serialize_compositeDeviceID_sequence_TLV_unfold compositeDeviceID;
-  (* Prf *) lemma_serialize_compositeDeviceID_sequence_TLV_size   compositeDeviceID; admit();
-  assert (length_of_opaque_serialization serialize_compositeDeviceID_sequence_TLV compositeDeviceID
-          == length_of_asn1_envelop_tag_with_TLV SEQUENCE serialize_compositeDeviceID compositeDeviceID)
-  // assert (length_of_opaque_serialization serialize_compositeDeviceID compositeDeviceID <= asn1_length_max - 6);
-  // assert (length_of_opaque_serialization serialize_compositeDeviceID_sequence_TLV compositeDeviceID <= asn1_length_max - 6)
-  // assert (let l = length_of_opaque_serialization serialize_compositeDeviceID compositeDeviceID in
-  //         length_of_opaque_serialization serialize_compositeDeviceID_sequence_TLV compositeDeviceID ==
-  //         1 + length_of_asn1_length (u l) + l)
-
-  let riot_extension: x509_extension_t serialize_compositeDeviceID_sequence_TLV = {
-    x509_extID       = OID_RIOT;
-    x509_extCritical = false;
-    x509_extValue    = compositeDeviceID
-  } in
-  (* Prf *) lemma_serialize_x509_extension_unfold
-            (* s *) serialize_compositeDeviceID_sequence_TLV
-            (* x *) riot_extension;
-  (* Prf *) lemma_serialize_x509_extension_size
-            (* s *) serialize_compositeDeviceID_sequence_TLV
-            (* x *) riot_extension;
-  (* Prf *) (**) lemma_serialize_asn1_oid_TLV_size riot_extension.x509_extID;
-  (* Prf *) (**) lemma_serialize_asn1_boolean_TLV_size riot_extension.x509_extCritical;
-  (* Prf *) lemma_serialize_x509_extension_sequence_TLV_size
-            (* s *) serialize_compositeDeviceID_sequence_TLV
-            (* x *) riot_extension;
-(* return *) riot_extension
