src/asn1/X509.Base.fst
@@ -10,22 +10,22 @@ open FStar.Integers
 
 module B32 = FStar.Bytes
 
-type cryptoAlg =
-| ECDSA_P256
-| ED25519
+type supported_crypto_alg_t =
+| AlgID_ECDSA_P256
+| AlgID_Ed25519
 
 unfold
 let pubkey_len
-  (pubkey_alg: cryptoAlg)
+  (pubkey_alg: supported_crypto_alg_t)
 = match pubkey_alg with
-  | ECDSA_P256 -> 32ul
-  | ED25519    -> 32ul
+  | AlgID_ECDSA_P256 -> 32ul
+  | AlgID_Ed25519    -> 32ul
 
 unfold
 let pubkey_t
-  (pubkey_alg: cryptoAlg)
+  (pubkey_alg: supported_crypto_alg_t)
 = match pubkey_alg with
-  | ECDSA_P256 -> datatype_of_asn1_type BIT_STRING
-  | ED25519    -> bs: datatype_of_asn1_type BIT_STRING
+  | AlgID_ECDSA_P256 -> datatype_of_asn1_type BIT_STRING
+  | AlgID_Ed25519    -> bs: datatype_of_asn1_type BIT_STRING
                      { bs.bs_len == 33ul /\
                        bs.bs_unused_bits == 0ul}
