src/asn1/X509.BasicFields.SubjectPublicKeyInfo.fst
@@ -16,40 +16,40 @@ open FStar.Integers
 *)
 /// Record repr
 type subjectPublicKeyInfo_t
-  (alg: cryptoAlg)
+  (alg: supported_crypto_alg_t)
 = { subjectPubKey_alg : algorithmIdentifier_t_inbound alg;
     subjectPubKey     : pubkey_t alg }
 
 let filter_subjectPublicKeyInfo_t'
-  (alg: cryptoAlg)
+  (alg: supported_crypto_alg_t)
   (x: (algorithmIdentifier_t_inbound alg) `tuple2` (datatype_of_asn1_type BIT_STRING))
 : GTot bool
 = match alg with
-  | ECDSA_P256 -> true
-  | ED25519    -> (snd x).bs_len = 33ul &&
+  | AlgID_ECDSA_P256 -> true
+  | AlgID_Ed25519    -> (snd x).bs_len = 33ul &&
                   (snd x).bs_unused_bits = 0ul
 
 /// tuple repr
 unfold
 let subjectPublicKeyInfo_t'
-  (alg: cryptoAlg)
+  (alg: supported_crypto_alg_t)
 = parse_filter_refine (filter_subjectPublicKeyInfo_t' alg)
 
 let synth_subjectPublicKeyInfo_t
-  (alg: cryptoAlg)
+  (alg: supported_crypto_alg_t)
   (x': subjectPublicKeyInfo_t' alg)
 : GTot (subjectPublicKeyInfo_t alg)
 = { subjectPubKey_alg = fst x';
     subjectPubKey     = snd x' }
 
 let synth_subjectPublicKeyInfo_t'
-  (alg: cryptoAlg)
+  (alg: supported_crypto_alg_t)
   (x: subjectPublicKeyInfo_t alg)
 : Tot (x': subjectPublicKeyInfo_t' alg { x == synth_subjectPublicKeyInfo_t alg x' })
 = (x.subjectPubKey_alg , x.subjectPubKey)
 
 let parse_subjectPublicKeyInfo
-  (alg: cryptoAlg)
+  (alg: supported_crypto_alg_t)
 : parser _ (subjectPublicKeyInfo_t alg)
 = parse_algorithmIdentifier_sequence_TLV alg
   `nondep_then`
@@ -60,7 +60,7 @@ let parse_subjectPublicKeyInfo
   synth_subjectPublicKeyInfo_t alg
 
 let serialize_subjectPublicKeyInfo
-  (alg: cryptoAlg)
+  (alg: supported_crypto_alg_t)
 : serializer (parse_subjectPublicKeyInfo alg)
 = serialize_synth
   (* p1 *) (parse_algorithmIdentifier_sequence_TLV alg
@@ -78,7 +78,7 @@ let serialize_subjectPublicKeyInfo
   (* prf*) ()
 
 let lemma_serialize_subjectPublicKeyInfo_unfold
-  (alg: cryptoAlg)
+  (alg: supported_crypto_alg_t)
   (x: subjectPublicKeyInfo_t alg)
 : Lemma (
   serialize (serialize_subjectPublicKeyInfo alg) x ==
@@ -107,7 +107,7 @@ let lemma_serialize_subjectPublicKeyInfo_unfold
   (* in *) x
 
 let lemma_serialize_subjectPublicKeyInfo_size
-  (alg: cryptoAlg)
+  (alg: supported_crypto_alg_t)
   (x: subjectPublicKeyInfo_t alg)
 : Lemma (
   Seq.length (serialize (serialize_subjectPublicKeyInfo alg) x) ==
@@ -117,31 +117,31 @@ let lemma_serialize_subjectPublicKeyInfo_size
 = lemma_serialize_subjectPublicKeyInfo_unfold alg x
 
 let subjectPublicKeyInfo_t_inbound
-  (alg: cryptoAlg)
+  (alg: supported_crypto_alg_t)
 = inbound_sequence_value_of (serialize_subjectPublicKeyInfo alg)
 
 /// TLV
 ///
 let parse_subjectPublicKeyInfo_sequence_TLV
-  (alg: cryptoAlg)
+  (alg: supported_crypto_alg_t)
 : parser _ (subjectPublicKeyInfo_t_inbound alg)
 = parse_asn1_sequence_TLV (serialize_subjectPublicKeyInfo alg)
 
 let serialize_subjectPublicKeyInfo_sequence_TLV
-  (alg: cryptoAlg)
+  (alg: supported_crypto_alg_t)
 : serializer (parse_subjectPublicKeyInfo_sequence_TLV alg)
 = serialize_asn1_sequence_TLV (serialize_subjectPublicKeyInfo alg)
 
 let lemma_serialize_subjectPublicKeyInfo_sequence_TLV_unfold
-  (alg: cryptoAlg)
+  (alg: supported_crypto_alg_t)
   (x: subjectPublicKeyInfo_t_inbound alg)
-: Lemma ( prop_serialize_asn1_sequence_TLV_unfold (serialize_subjectPublicKeyInfo alg) x )
+: Lemma ( predicate_serialize_asn1_sequence_TLV_unfold (serialize_subjectPublicKeyInfo alg) x )
 = lemma_serialize_asn1_sequence_TLV_unfold (serialize_subjectPublicKeyInfo alg) x
 
 let lemma_serialize_subjectPublicKeyInfo_sequence_TLV_size
-  (alg: cryptoAlg)
+  (alg: supported_crypto_alg_t)
   (x: subjectPublicKeyInfo_t_inbound alg)
-: Lemma ( prop_serialize_asn1_sequence_TLV_size (serialize_subjectPublicKeyInfo alg) x )
+: Lemma ( predicate_serialize_asn1_sequence_TLV_size (serialize_subjectPublicKeyInfo alg) x )
 = lemma_serialize_asn1_sequence_TLV_size (serialize_subjectPublicKeyInfo alg) x
 
 (* NOTE: For a subjectPublicKeyInfo for Ed25519, it consists
@@ -168,21 +168,21 @@ let lemma_serialize_subjectPublicKeyInfo_sequence_TLV_size
 
 #push-options "--query_stats --z3rlimit 32"
 let lemma_serialize_subjectPublicKeyInfo_sequence_TLV_size_exact
-  (alg: cryptoAlg {alg == ED25519})
+  (alg: supported_crypto_alg_t {alg == AlgID_Ed25519})
   (x: subjectPublicKeyInfo_t_inbound alg)
 : Lemma (
   match alg with
-  | ED25519   -> ( length_of_opaque_serialization (serialize_subjectPublicKeyInfo_sequence_TLV alg) x == 44 )
+  | AlgID_Ed25519   -> ( length_of_opaque_serialization (serialize_subjectPublicKeyInfo_sequence_TLV alg) x == 44 )
 )
 =
   match alg with
-  | ED25519   -> ( (* reveal the SEQUENCE envelop *)
+  | AlgID_Ed25519   -> ( (* reveal the SEQUENCE envelop *)
                    lemma_serialize_subjectPublicKeyInfo_sequence_TLV_unfold alg x;
                    lemma_serialize_subjectPublicKeyInfo_sequence_TLV_size   alg x;
                      (* reveal the SEQUENCE body *)
                      lemma_serialize_subjectPublicKeyInfo_size alg x;
                      (**) lemma_serialize_algorithmIdentifier_sequence_TLV_size_exact alg x.subjectPubKey_alg;
-                     assert ( let bs: pubkey_t ED25519 = x.subjectPubKey in
+                     assert ( let bs: pubkey_t AlgID_Ed25519 = x.subjectPubKey in
                               length_of_asn1_primitive_TLV bs == 35 );
                      () )
 #pop-options
@@ -192,7 +192,7 @@ let lemma_serialize_subjectPublicKeyInfo_sequence_TLV_size_exact
 
 inline_for_extraction
 let serialize32_subjectPublicKeyInfo_backwards
-  (alg: cryptoAlg)
+  (alg: supported_crypto_alg_t)
 : serializer32_backwards (serialize_subjectPublicKeyInfo alg)
 = serialize32_synth_backwards
   (* ls *) (serialize32_algorithmIdentifier_sequence_TLV_backwards alg
@@ -206,7 +206,7 @@ let serialize32_subjectPublicKeyInfo_backwards
   (* prf*) ()
 
 let serialize32_subjectPublicKeyInfo_sequence_TLV_backwards
-  (alg: cryptoAlg)
+  (alg: supported_crypto_alg_t)
 : serializer32_backwards (serialize_subjectPublicKeyInfo_sequence_TLV alg)
 = serialize32_asn1_sequence_TLV_backwards
   (* ls *) (serialize32_subjectPublicKeyInfo_backwards alg)
@@ -217,20 +217,20 @@ let _ = assert (length_of_oid OID_EC_GRP_SECP256R1 == 6)
 module B32 = FStar.Bytes
 open X509.Crypto.AlgorithmIdentifier
 let subjectPublicKeyInfo_raw_t
-  (alg: cryptoAlg{alg == ED25519})
+  (alg: supported_crypto_alg_t{alg == AlgID_Ed25519})
 = match alg with
-  | ED25519   -> B32.lbytes32 32ul
+  | AlgID_Ed25519   -> B32.lbytes32 32ul
 
-#push-options "--query_stats --z3rlimit 8 --fuel 2 --ifuel 1"
+#push-options "--z3rlimit 16 --fuel 2 --ifuel 1"
 let x509_get_subjectPublicKeyInfo
-  (pubkey_alg: cryptoAlg {pubkey_alg == ED25519} )
+  (pubkey_alg: supported_crypto_alg_t {pubkey_alg == AlgID_Ed25519} )
   (pubkey: B32.lbytes32 32ul)
 : Tot (subjectPublicKeyInfo_t_inbound pubkey_alg)
 =
   lemma_trivial_bit_string_is_valid 33ul pubkey;
   let pubkey_bs: pubkey_t pubkey_alg = Mkbit_string_t 33ul 0ul pubkey in
 
-  if (pubkey_alg = ED25519) then
+  if (pubkey_alg = AlgID_Ed25519) then
   ( let alg_id: algorithmIdentifier_t_inbound pubkey_alg = x509_get_algorithmIdentifier pubkey_alg in
     (* Prf *) lemma_serialize_algorithmIdentifier_sequence_TLV_size_exact pubkey_alg alg_id;
 
