src/asn1/X509.Crypto.AlgorithmIdentifier.fst
@@ -28,80 +28,80 @@ type algorithmIdentifier_Ed25519_t = {
 }
 
 let algorithmIdentifier_t
-  (alg: cryptoAlg)
+  (alg: supported_crypto_alg_t)
 = match alg with
-  | ECDSA_P256 -> algorithmIdentifier_ECDSA_P256_t
-  | ED25519    -> algorithmIdentifier_Ed25519_t
+  | AlgID_ECDSA_P256 -> algorithmIdentifier_ECDSA_P256_t
+  | AlgID_Ed25519    -> algorithmIdentifier_Ed25519_t
 
 private
 let algorithmIdentifier_t'_aux
-  (alg: cryptoAlg)
+  (alg: supported_crypto_alg_t)
 = match alg with
-  | ECDSA_P256 -> tuple2 (datatype_of_asn1_type OID) (datatype_of_asn1_type OID)
-  | ED25519    -> datatype_of_asn1_type OID
+  | AlgID_ECDSA_P256 -> tuple2 (datatype_of_asn1_type OID) (datatype_of_asn1_type OID)
+  | AlgID_Ed25519    -> datatype_of_asn1_type OID
 
 /// tuple repr
 let filter_algorithmIdentifier_t'
-  (alg: cryptoAlg)
+  (alg: supported_crypto_alg_t)
   (x': algorithmIdentifier_t'_aux alg)
 : GTot bool
 = match alg with
-  | ECDSA_P256 -> ( let x' = x' <: tuple2 (datatype_of_asn1_type OID) (datatype_of_asn1_type OID) in
+  | AlgID_ECDSA_P256 -> ( let x' = x' <: tuple2 (datatype_of_asn1_type OID) (datatype_of_asn1_type OID) in
                     fst x' = OID_EC_ALG_UNRESTRICTED &&
                     snd x' = OID_EC_GRP_SECP256R1 )
-  | ED25519    -> ( let x' = x'<: datatype_of_asn1_type OID in
+  | AlgID_Ed25519    -> ( let x' = x'<: datatype_of_asn1_type OID in
                     x' = OID_ED25519 )
 
 let algorithmIdentifier_t'
-  (alg: cryptoAlg)
+  (alg: supported_crypto_alg_t)
 = parse_filter_refine (filter_algorithmIdentifier_t' alg)
 
 /// tuple repr -> record repr
 let synth_algorithmIdentifier_t
-  (alg: cryptoAlg)
+  (alg: supported_crypto_alg_t)
   (x': algorithmIdentifier_t' alg)
 : GTot (algorithmIdentifier_t alg)
 = match alg with
-  | ECDSA_P256 -> ( let x' = x' <: tuple2 (datatype_of_asn1_type OID) (datatype_of_asn1_type OID) in
+  | AlgID_ECDSA_P256 -> ( let x' = x' <: tuple2 (datatype_of_asn1_type OID) (datatype_of_asn1_type OID) in
                     { alg_id_oid_ecdsa = fst x';
                       alg_id_oid_p256  = snd x' } )
-  | ED25519    -> ( let x' = x' <: datatype_of_asn1_type OID in
+  | AlgID_Ed25519    -> ( let x' = x' <: datatype_of_asn1_type OID in
                     { algID_ed25519 = x' } )
 
 /// record repr -> tuple repr
 let synth_algorithmIdentifier_t'
-  (alg: cryptoAlg)
+  (alg: supported_crypto_alg_t)
   (x: algorithmIdentifier_t alg)
 : Tot (x': algorithmIdentifier_t' alg { x == synth_algorithmIdentifier_t alg x' })
 = match alg with
-  | ECDSA_P256 -> ( let x = x <: algorithmIdentifier_ECDSA_P256_t in
+  | AlgID_ECDSA_P256 -> ( let x = x <: algorithmIdentifier_ECDSA_P256_t in
                     ((x.alg_id_oid_ecdsa <: datatype_of_asn1_type OID),
                      (x.alg_id_oid_p256  <: datatype_of_asn1_type OID)) )
-  | ED25519    -> ( let x = x<: algorithmIdentifier_Ed25519_t in
+  | AlgID_Ed25519    -> ( let x = x<: algorithmIdentifier_Ed25519_t in
                     x.algID_ed25519 )
 
 let parse_algorithmIdentifier_kind
-  (alg: cryptoAlg)
+  (alg: supported_crypto_alg_t)
 : parser_kind
 = match alg with
-  | ECDSA_P256 -> ( parse_asn1_TLV_kind_of_type OID
+  | AlgID_ECDSA_P256 -> ( parse_asn1_TLV_kind_of_type OID
                     `and_then_kind`
                     parse_asn1_TLV_kind_of_type OID )
-  | ED25519    -> ( parse_asn1_TLV_kind_of_type OID )
+  | AlgID_Ed25519    -> ( parse_asn1_TLV_kind_of_type OID )
 
 /// sequence value (body) parser
 let parse_algorithmIdentifier
-  (alg: cryptoAlg)
+  (alg: supported_crypto_alg_t)
 : parser (parse_algorithmIdentifier_kind alg) (algorithmIdentifier_t alg)
 = match alg with
-  | ECDSA_P256 -> ( parse_asn1_TLV_of_type OID
+  | AlgID_ECDSA_P256 -> ( parse_asn1_TLV_of_type OID
                     `nondep_then`
                     parse_asn1_TLV_of_type OID
                     `parse_filter`
                     filter_algorithmIdentifier_t' alg
                     `parse_synth`
                     synth_algorithmIdentifier_t alg )
-  | ED25519    -> ( parse_asn1_TLV_of_type OID
+  | AlgID_Ed25519    -> ( parse_asn1_TLV_of_type OID
                     `parse_filter`
                     filter_algorithmIdentifier_t' alg
                     `parse_synth`
@@ -109,10 +109,10 @@ let parse_algorithmIdentifier
 
 /// sequence value serializer
 let serialize_algorithmIdentifier
-  (alg: cryptoAlg)
+  (alg: supported_crypto_alg_t)
 : serializer (parse_algorithmIdentifier alg)
 = match alg with
-  | ECDSA_P256 -> ( serialize_synth
+  | AlgID_ECDSA_P256 -> ( serialize_synth
                     (* p1 *) (parse_asn1_TLV_of_type OID
                               `nondep_then`
                               parse_asn1_TLV_of_type OID
@@ -127,7 +127,7 @@ let serialize_algorithmIdentifier
                     (* g1 *) (synth_algorithmIdentifier_t' alg)
                     (* prf*) () )
 
-  | ED25519    -> ( serialize_synth
+  | AlgID_Ed25519    -> ( serialize_synth
                     (* p1 *) (parse_asn1_TLV_of_type OID
                               `parse_filter`
                               filter_algorithmIdentifier_t' alg)
@@ -140,21 +140,21 @@ let serialize_algorithmIdentifier
 
 /// lemma: unfold sequence value serializer
 let lemma_serialize_algorithmIdentifier_unfold
-  (alg: cryptoAlg)
+  (alg: supported_crypto_alg_t)
   (x: algorithmIdentifier_t alg)
 : Lemma (
   match alg with
-  | ECDSA_P256 -> ( serialize (serialize_algorithmIdentifier alg) x ==
+  | AlgID_ECDSA_P256 -> ( serialize (serialize_algorithmIdentifier alg) x ==
                     serialize (serialize_asn1_TLV_of_type OID) OID_EC_ALG_UNRESTRICTED
                     `Seq.append`
                     serialize (serialize_asn1_TLV_of_type OID) OID_EC_GRP_SECP256R1 )
-  | ED25519    -> ( serialize (serialize_algorithmIdentifier alg) x ==
+  | AlgID_Ed25519    -> ( serialize (serialize_algorithmIdentifier alg) x ==
                     serialize (serialize_asn1_TLV_of_type OID) OID_ED25519 /\
                     length_of_opaque_serialization (serialize_algorithmIdentifier alg) x ==
                     5
                     ))
 = match alg with
-  | ECDSA_P256 -> ( serialize_nondep_then_eq
+  | AlgID_ECDSA_P256 -> ( serialize_nondep_then_eq
                     (* s1 *) (serialize_asn1_TLV_of_type OID)
                     (* s2 *) (serialize_asn1_TLV_of_type OID)
                     (* in *) (synth_algorithmIdentifier_t' alg x);
@@ -173,7 +173,7 @@ let lemma_serialize_algorithmIdentifier_unfold
                     (* g1 *) (synth_algorithmIdentifier_t' alg)
                     (* prf*) ()
                     (* in *) x )
-  | ED25519    -> ( serialize_synth_eq
+  | AlgID_Ed25519    -> ( serialize_synth_eq
                     (* p1 *) (parse_asn1_TLV_of_type OID
                               `parse_filter`
                               filter_algorithmIdentifier_t' alg)
@@ -190,15 +190,15 @@ let lemma_serialize_algorithmIdentifier_unfold
 
 #push-options "--query_stats"
 let lemma_serialize_algorithmIdentifier_size
-  (alg: cryptoAlg)
+  (alg: supported_crypto_alg_t)
   (x: algorithmIdentifier_t alg)
 : Lemma (
   match alg with (* FIXME *)
-  // | ECDSA_P256 -> ( let x = x <: algorithmIdentifier_ECDSA_P256_t in
+  // | AlgID_ECDSA_P256 -> ( let x = x <: algorithmIdentifier_ECDSA_P256_t in
   //                   Seq.length (serialize (serialize_algorithmIdentifier alg) x) ==
   //                   length_of_asn1_primitive_TLV x.alg_id_oid_ecdsa +
   //                   length_of_asn1_primitive_TLV x.alg_id_oid_p256 )
-  | ED25519    -> ( let x = x <: algorithmIdentifier_Ed25519_t in
+  | AlgID_Ed25519    -> ( let x = x <: algorithmIdentifier_Ed25519_t in
                     Seq.length (serialize (serialize_algorithmIdentifier alg) x) ==
                     5 )
                     //length_of_asn1_primitive_TLV x.algID_ed25519 /\
@@ -206,63 +206,63 @@ let lemma_serialize_algorithmIdentifier_size
                     //length_of_asn1_primitive_TLV x.algID_ed25519 == 5)
   | _ -> True)
 = match alg with
-  | ECDSA_P256 -> ( lemma_serialize_algorithmIdentifier_unfold alg x )
-  | ED25519    -> ( lemma_serialize_algorithmIdentifier_unfold alg x;
+  | AlgID_ECDSA_P256 -> ( lemma_serialize_algorithmIdentifier_unfold alg x )
+  | AlgID_Ed25519    -> ( lemma_serialize_algorithmIdentifier_unfold alg x;
                     assert_norm (length_of_asn1_primitive_TLV x.algID_ed25519 == 5 ))
 
 /// inbound record repr
 let algorithmIdentifier_t_inbound
-  (alg: cryptoAlg)
+  (alg: supported_crypto_alg_t)
 = match alg with
-  | ECDSA_P256 -> inbound_sequence_value_of (serialize_algorithmIdentifier alg)
-  | ED25519    -> inbound_sequence_value_of (serialize_algorithmIdentifier alg)
+  | AlgID_ECDSA_P256 -> inbound_sequence_value_of (serialize_algorithmIdentifier alg)
+  | AlgID_Ed25519    -> inbound_sequence_value_of (serialize_algorithmIdentifier alg)
 
 /// TLV
 // unfold
 let parse_algorithmIdentifier_sequence_TLV
-  (alg: cryptoAlg)
+  (alg: supported_crypto_alg_t)
 : parser (parse_asn1_envelop_tag_with_TLV_kind SEQUENCE) (algorithmIdentifier_t_inbound alg)
 = match alg with
-  | ECDSA_P256 -> ( //algorithmIdentifier_t_inbound alg
+  | AlgID_ECDSA_P256 -> ( //algorithmIdentifier_t_inbound alg
                     //`coerce_parser`
                     parse_asn1_sequence_TLV (serialize_algorithmIdentifier alg) )
-  | ED25519    -> ( //algorithmIdentifier_t_inbound alg
+  | AlgID_Ed25519    -> ( //algorithmIdentifier_t_inbound alg
                     //`coerce_parser`
                     parse_asn1_sequence_TLV (serialize_algorithmIdentifier alg) )
 
 let serialize_algorithmIdentifier_sequence_TLV
-  (alg: cryptoAlg)
+  (alg: supported_crypto_alg_t)
 : serializer (parse_algorithmIdentifier_sequence_TLV alg)
 = match alg with
-  | ECDSA_P256 -> ( serialize_asn1_sequence_TLV (serialize_algorithmIdentifier alg) )
-  | ED25519    -> ( serialize_asn1_sequence_TLV (serialize_algorithmIdentifier alg) )
+  | AlgID_ECDSA_P256 -> ( serialize_asn1_sequence_TLV (serialize_algorithmIdentifier alg) )
+  | AlgID_Ed25519    -> ( serialize_asn1_sequence_TLV (serialize_algorithmIdentifier alg) )
 
 let lemma_serialize_algorithmIdentifier_sequence_TLV_unfold
-  (alg: cryptoAlg)
+  (alg: supported_crypto_alg_t)
   (x: algorithmIdentifier_t_inbound alg)
-: Lemma ( prop_serialize_asn1_sequence_TLV_unfold (serialize_algorithmIdentifier alg) x )
+: Lemma ( predicate_serialize_asn1_sequence_TLV_unfold (serialize_algorithmIdentifier alg) x )
 = lemma_serialize_asn1_sequence_TLV_unfold (serialize_algorithmIdentifier alg) x
 
 let lemma_serialize_algorithmIdentifier_sequence_TLV_size
-  (alg: cryptoAlg)
+  (alg: supported_crypto_alg_t)
   (x: algorithmIdentifier_t_inbound alg)
-: Lemma ( prop_serialize_asn1_sequence_TLV_size (serialize_algorithmIdentifier alg) x )
+: Lemma ( predicate_serialize_asn1_sequence_TLV_size (serialize_algorithmIdentifier alg) x )
 = match alg with
-  | ECDSA_P256 -> ( lemma_serialize_asn1_sequence_TLV_size (serialize_algorithmIdentifier alg) x )
-  | ED25519    -> ( lemma_serialize_asn1_sequence_TLV_size (serialize_algorithmIdentifier alg) x )
+  | AlgID_ECDSA_P256 -> ( lemma_serialize_asn1_sequence_TLV_size (serialize_algorithmIdentifier alg) x )
+  | AlgID_Ed25519    -> ( lemma_serialize_asn1_sequence_TLV_size (serialize_algorithmIdentifier alg) x )
 
 #push-options "--query_stats --z3rlimit 32 --fuel 4 --ifuel 4"
 let lemma_serialize_algorithmIdentifier_sequence_TLV_size_exact
-  (alg: cryptoAlg {alg == ED25519})
+  (alg: supported_crypto_alg_t {alg == AlgID_Ed25519})
   (x: algorithmIdentifier_t alg)
 : Lemma (
   match alg with
-  // | ECDSA_P256 -> ( length_of_opaque_serialization (serialize_algorithmIdentifier_sequence_TLV alg) x == 17 )
-  | ED25519    -> ( lemma_serialize_algorithmIdentifier_size alg x;
+  // | AlgID_ECDSA_P256 -> ( length_of_opaque_serialization (serialize_algorithmIdentifier_sequence_TLV alg) x == 17 )
+  | AlgID_Ed25519    -> ( lemma_serialize_algorithmIdentifier_size alg x;
                     length_of_opaque_serialization (serialize_algorithmIdentifier_sequence_TLV alg) x == 7 )
 )
 = match alg with
-  | ED25519    -> ( lemma_serialize_algorithmIdentifier_size alg x;
+  | AlgID_Ed25519    -> ( lemma_serialize_algorithmIdentifier_size alg x;
                     lemma_serialize_asn1_sequence_TLV_unfold (serialize_algorithmIdentifier alg) x;
                     lemma_serialize_asn1_sequence_TLV_size   (serialize_algorithmIdentifier alg) x;
                     // lemma_serialize_algorithmIdentifier_size alg x;
@@ -274,10 +274,10 @@ let lemma_serialize_algorithmIdentifier_sequence_TLV_size_exact
 
 inline_for_extraction
 let serialize32_algorithmIdentifier_backwards
-  (alg: cryptoAlg)
+  (alg: supported_crypto_alg_t)
 : serializer32_backwards (serialize_algorithmIdentifier alg)
 = match alg with
-  | ECDSA_P256 -> ( serialize32_synth_backwards
+  | AlgID_ECDSA_P256 -> ( serialize32_synth_backwards
                     (* ls *) (serialize32_asn1_TLV_backwards_of_type OID
                               `serialize32_nondep_then_backwards`
                               serialize32_asn1_TLV_backwards_of_type OID
@@ -287,7 +287,7 @@ let serialize32_algorithmIdentifier_backwards
                     (* g1 *) (synth_algorithmIdentifier_t' alg)
                     (* g1'*) (synth_algorithmIdentifier_t' alg)
                     (* prf*) () )
-  | ED25519    -> ( serialize32_synth_backwards
+  | AlgID_Ed25519    -> ( serialize32_synth_backwards
                     (* ls *) (serialize32_asn1_TLV_backwards_of_type OID
                               `serialize32_filter_backwards`
                               filter_algorithmIdentifier_t' alg)
@@ -297,12 +297,12 @@ let serialize32_algorithmIdentifier_backwards
                     (* prf*) () )
 
 let serialize32_algorithmIdentifier_sequence_TLV_backwards
-  (alg: cryptoAlg)
+  (alg: supported_crypto_alg_t)
 : serializer32_backwards (serialize_algorithmIdentifier_sequence_TLV alg)
 = match alg with
-  | ECDSA_P256 -> ( serialize32_asn1_sequence_TLV_backwards
+  | AlgID_ECDSA_P256 -> ( serialize32_asn1_sequence_TLV_backwards
                     (* s32 *) (serialize32_algorithmIdentifier_backwards alg) )
-  | ED25519    -> ( serialize32_asn1_sequence_TLV_backwards
+  | AlgID_Ed25519    -> ( serialize32_asn1_sequence_TLV_backwards
                     (* s32 *) (serialize32_algorithmIdentifier_backwards alg) )
 
 (* helpers *)
@@ -311,11 +311,11 @@ let _ = assert (length_of_oid OID_EC_GRP_SECP256R1 == 6)
 #push-options "--z3rlimit 4 --fuel 2 --ifuel 1"
 noextract inline_for_extraction
 let x509_get_algorithmIdentifier
-  (alg: cryptoAlg {alg == ED25519})
+  (alg: supported_crypto_alg_t {alg == AlgID_Ed25519})
 : Tot (algorithmIdentifier_t_inbound alg)
 =
   match alg with
-  | ED25519 -> ( let algID: algorithmIdentifier_t alg = { algID_ed25519 = OID_ED25519 } in
+  | AlgID_Ed25519 -> ( let algID: algorithmIdentifier_t alg = { algID_ed25519 = OID_ED25519 } in
                  (* Prf *) lemma_serialize_algorithmIdentifier_size alg algID;
                  (* Prf *) (**) lemma_serialize_asn1_oid_TLV_size algID.algID_ed25519;
                  (* return *) algID )
