src/asn1/X509.Crypto.Signature.fst
@@ -14,46 +14,46 @@ module B32 = FStar.Bytes
 open ASN1.Base
 
 let x509_signature_t_aux
-  (alg: cryptoAlg {alg == ED25519})
+  (alg: supported_crypto_alg_t {alg == AlgID_Ed25519})
 = match alg with
-  | ED25519   -> datatype_of_asn1_type BIT_STRING
+  | AlgID_Ed25519   -> datatype_of_asn1_type BIT_STRING
 
 let filter_x509_signature
-  (alg: cryptoAlg {alg == ED25519})
+  (alg: supported_crypto_alg_t {alg == AlgID_Ed25519})
   (x: x509_signature_t_aux alg)
 : GTot (bool)
 = match alg with
-  | ED25519   -> ( let x = x <: datatype_of_asn1_type BIT_STRING in
+  | AlgID_Ed25519   -> ( let x = x <: datatype_of_asn1_type BIT_STRING in
                    x.bs_len = 65ul &&
                    x.bs_unused_bits = 0ul )
 
 let x509_signature_t
-  (alg: cryptoAlg {alg == ED25519})
+  (alg: supported_crypto_alg_t {alg == AlgID_Ed25519})
 = match alg with
-  | ED25519   -> ( bs: datatype_of_asn1_type BIT_STRING
+  | AlgID_Ed25519   -> ( bs: datatype_of_asn1_type BIT_STRING
                        { v bs.bs_len == 65 /\
                          v bs.bs_unused_bits == 0 })
 
 let parse_x509_signature_kind
-  (alg: cryptoAlg {alg == ED25519})
+  (alg: supported_crypto_alg_t {alg == AlgID_Ed25519})
 = match alg with
-  | ED25519   -> parse_asn1_TLV_kind_of_type BIT_STRING
+  | AlgID_Ed25519   -> parse_asn1_TLV_kind_of_type BIT_STRING
 
 let parse_x509_signature
-  (alg: cryptoAlg {alg == ED25519})
+  (alg: supported_crypto_alg_t {alg == AlgID_Ed25519})
 : parser (parse_x509_signature_kind alg) (x509_signature_t alg)
 = match alg with
-  | ED25519   -> ( parse_asn1_TLV_of_type BIT_STRING
+  | AlgID_Ed25519   -> ( parse_asn1_TLV_of_type BIT_STRING
                    `parse_filter`
                    filter_x509_signature alg
                    `parse_synth`
                    (fun x -> x <: x509_signature_t alg))
 
 let serialize_x509_signature
-  (alg: cryptoAlg {alg == ED25519})
+  (alg: supported_crypto_alg_t {alg == AlgID_Ed25519})
 : serializer (parse_x509_signature alg)
 = match alg with
-  | ED25519   -> ( serialize_synth
+  | AlgID_Ed25519   -> ( serialize_synth
                    (* p1 *) (parse_asn1_TLV_of_type BIT_STRING
                              `parse_filter`
                              filter_x509_signature alg)
@@ -65,11 +65,11 @@ let serialize_x509_signature
                    (* prf*) () )
 
 let lemma_serialize_x509_signature_unfold
-  (alg: cryptoAlg {alg == ED25519})
+  (alg: supported_crypto_alg_t {alg == AlgID_Ed25519})
   (x: x509_signature_t alg)
 : Lemma (
   match alg with
-  | ED25519   -> ( serialize_x509_signature alg `serialize` x ==
+  | AlgID_Ed25519   -> ( serialize_x509_signature alg `serialize` x ==
                    serialize_asn1_TLV_of_type BIT_STRING x )
 )
 = serialize_synth_eq
@@ -85,68 +85,68 @@ let lemma_serialize_x509_signature_unfold
   (* in *) x
 
 let lemma_serialize_x509_signature_size
-  (alg: cryptoAlg {alg == ED25519})
+  (alg: supported_crypto_alg_t {alg == AlgID_Ed25519})
   (x: x509_signature_t alg)
 : Lemma (
   match alg with
-  | ED25519   -> ( length_of_opaque_serialization (serialize_x509_signature alg) x ==
+  | AlgID_Ed25519   -> ( length_of_opaque_serialization (serialize_x509_signature alg) x ==
                    length_of_asn1_primitive_TLV #BIT_STRING x /\
                    length_of_opaque_serialization (serialize_x509_signature alg) x == 67 )
 )
 = match alg with
-  | ED25519   -> ( lemma_serialize_x509_signature_unfold alg x;
+  | AlgID_Ed25519   -> ( lemma_serialize_x509_signature_unfold alg x;
                    lemma_serialize_asn1_bit_string_TLV_size x )
 
 let x509_signature_t_inbound
-  (alg: cryptoAlg {alg == ED25519})
+  (alg: supported_crypto_alg_t {alg == AlgID_Ed25519})
 = match alg with
-  | ED25519   -> ( inbound_sequence_value_of (serialize_x509_signature alg) )
+  | AlgID_Ed25519   -> ( inbound_sequence_value_of (serialize_x509_signature alg) )
 
 let parse_x509_signature_sequence_TLV
-  (alg: cryptoAlg {alg == ED25519})
+  (alg: supported_crypto_alg_t {alg == AlgID_Ed25519})
 : parser _ (x509_signature_t_inbound alg)
 = match alg with
-  | ED25519   -> ( parse_asn1_sequence_TLV (serialize_x509_signature alg) )
+  | AlgID_Ed25519   -> ( parse_asn1_sequence_TLV (serialize_x509_signature alg) )
 
 let serialize_x509_signature_sequence_TLV
-  (alg: cryptoAlg {alg == ED25519})
+  (alg: supported_crypto_alg_t {alg == AlgID_Ed25519})
 : serializer (parse_x509_signature_sequence_TLV alg)
 = match alg with
-  | ED25519   -> ( serialize_asn1_sequence_TLV (serialize_x509_signature alg) )
+  | AlgID_Ed25519   -> ( serialize_asn1_sequence_TLV (serialize_x509_signature alg) )
 
 let lemma_serialize_x509_signature_sequence_TLV_unfold
-  (alg: cryptoAlg {alg == ED25519})
+  (alg: supported_crypto_alg_t {alg == AlgID_Ed25519})
   (x: x509_signature_t_inbound alg)
-: Lemma ( prop_serialize_asn1_sequence_TLV_unfold (serialize_x509_signature alg) x )
+: Lemma ( predicate_serialize_asn1_sequence_TLV_unfold (serialize_x509_signature alg) x )
 = match alg with
-  | ED25519   -> ( lemma_serialize_asn1_sequence_TLV_unfold (serialize_x509_signature alg) x )
+  | AlgID_Ed25519   -> ( lemma_serialize_asn1_sequence_TLV_unfold (serialize_x509_signature alg) x )
 
 let lemma_serialize_x509_signature_sequence_TLV_size
-  (alg: cryptoAlg {alg == ED25519})
+  (alg: supported_crypto_alg_t {alg == AlgID_Ed25519})
   (x: x509_signature_t_inbound alg)
-: Lemma ( prop_serialize_asn1_sequence_TLV_size (serialize_x509_signature alg) x )
+: Lemma ( predicate_serialize_asn1_sequence_TLV_size (serialize_x509_signature alg) x )
 = match alg with
-  | ED25519   -> ( lemma_serialize_asn1_sequence_TLV_size (serialize_x509_signature alg) x )
+  | AlgID_Ed25519   -> ( lemma_serialize_asn1_sequence_TLV_size (serialize_x509_signature alg) x )
 
 #push-options "--z3rlimit 32 --fuel 4 --ifuel 4"
 let lemma_serialize_x509_signature_sequence_TLV_size_exact
-  (alg: cryptoAlg {alg == ED25519})
+  (alg: supported_crypto_alg_t {alg == AlgID_Ed25519})
   (x: x509_signature_t_inbound alg)
 : Lemma (
   match alg with
-  | ED25519    -> ( length_of_opaque_serialization (serialize_x509_signature_sequence_TLV alg) x == 69 )
+  | AlgID_Ed25519    -> ( length_of_opaque_serialization (serialize_x509_signature_sequence_TLV alg) x == 69 )
 )
 = match alg with
-  | ED25519    -> ( lemma_serialize_x509_signature_sequence_TLV_size alg x;
+  | AlgID_Ed25519    -> ( lemma_serialize_x509_signature_sequence_TLV_size alg x;
                     lemma_serialize_x509_signature_size alg x )
 #pop-options
 
 (* Low *)
 let serialize32_x509_signature_backwards
-  (alg: cryptoAlg {alg == ED25519})
+  (alg: supported_crypto_alg_t {alg == AlgID_Ed25519})
 : serializer32_backwards (serialize_x509_signature alg)
 = match alg with
-  | ED25519   -> ( serialize32_synth_backwards
+  | AlgID_Ed25519   -> ( serialize32_synth_backwards
                    (* s32 *) (serialize32_asn1_bit_string_TLV_backwards ()
                               `serialize32_filter_backwards`
                               filter_x509_signature alg)
@@ -156,10 +156,10 @@ let serialize32_x509_signature_backwards
                    (* prf *) () )
 
 let serialize32_x509_signature_sequence_TLV_backwards
-  (alg: cryptoAlg {alg == ED25519})
+  (alg: supported_crypto_alg_t {alg == AlgID_Ed25519})
 : serializer32_backwards (serialize_x509_signature_sequence_TLV alg)
 = match alg with
-  | ED25519   -> ( serialize32_asn1_sequence_TLV_backwards (serialize32_x509_signature_backwards alg) )
+  | AlgID_Ed25519   -> ( serialize32_asn1_sequence_TLV_backwards (serialize32_x509_signature_backwards alg) )
 
 
 (* Helpers *)
@@ -167,16 +167,16 @@ let _ = assert (length_of_oid OID_EC_GRP_SECP256R1 == 6)
 
 module B32 = FStar.Bytes
 let x509_signature_raw_t
-  (alg: cryptoAlg {alg == ED25519})
+  (alg: supported_crypto_alg_t {alg == AlgID_Ed25519})
 = match alg with
-  | ED25519   -> ( B32.lbytes32 64ul )
+  | AlgID_Ed25519   -> ( B32.lbytes32 64ul )
 
 let x509_get_signature
-  (alg: cryptoAlg {alg == ED25519})
+  (alg: supported_crypto_alg_t {alg == AlgID_Ed25519})
   (sig32: x509_signature_raw_t alg)
 : Tot (x509_signature_t_inbound alg)
 =
   match alg with
-  | ED25519   -> ( let sig_bs: x509_signature_t alg = Mkbit_string_t 65ul 0ul sig32 in
+  | AlgID_Ed25519   -> ( let sig_bs: x509_signature_t alg = Mkbit_string_t 65ul 0ul sig32 in
                    (* Prf *) lemma_serialize_x509_signature_size alg sig_bs;
                    (* return *) sig_bs )
